examples/dm4all/ExnHandleTwoPostCond.fst
@@ -20,7 +20,7 @@ let return_wp (a:Type) (x:a) : wp_type a = fun p q -> p x
 unfold
 let bind_wp (_ : range) (a : Type) (b : Type) (wp : wp_type a) (f : a -> wp_type b) =
   fun p q -> wp (fun x -> f x p q) (fun e -> q e)
-  
+
 let interp (#a:Type) (c : repr a) : wp_type a = fun p q ->
   match c with
   | Inl x -> p x
@@ -49,7 +49,7 @@ let raise #a e = EXC?.reflect (Inr e)
 (* The algebra extension operation is inlined for better readability *)
 
 unfold
-let rep_try_catch (#a:Type) 
+let rep_try_catch (#a:Type)
                   (#b:Type)
                   (c1:repr a)
                   (h_c:exn -> repr b)
@@ -64,36 +64,36 @@ let wp_return (#a:Type) (x:a) : wp_type a = fun p q -> p x
 unfold
 let wp_bind (#a:Type) (#b:Type) (wp : wp_type a) (f : a -> wp_type b) =
   fun p q -> wp (fun x -> f x p q) (fun e -> q e)
-  
+
 unfold
 let wp_raise (#a:Type) (e:exn) : wp_type a = fun p q -> q e
 
 unfold
-let wp_try_catch (#a:Type) 
-                 (#b:Type) 
-                 (wp1:wp_type a) 
-                 (h_wp:exn -> wp_type b) 
-                 (wp2:a -> wp_type b) : wp_type b = 
+let wp_try_catch (#a:Type)
+                 (#b:Type)
+                 (wp1:wp_type a)
+                 (h_wp:exn -> wp_type b)
+                 (wp2:a -> wp_type b) : wp_type b =
   fun p q -> wp1 (fun x -> wp2 x p q) (fun e -> h_wp e p q)
 
 (* We should get this from the framework FIXME *)
 assume val reify_related (#a #b:Type) (wp:_) (c : (x:a -> EXC b (wp x))) :
                          Lemma (forall (x:a). EXC?.mrelation (reify (c x)) (wp x))
 
-let lemma_try_catch (#a:Type) 
-                    (#b:Type) 
+let lemma_try_catch (#a:Type)
+                    (#b:Type)
                     (wp1:wp_type a)
                     (c1:either a exn)
-                    (h_wp:exn -> wp_type b) 
+                    (h_wp:exn -> wp_type b)
                     (h_c:(e:exn -> either b exn))
-                    (wp2:a -> wp_type b) 
+                    (wp2:a -> wp_type b)
                     (c2:(x:a -> either b exn))
   : Lemma (requires ((EXC?.mrelation c1 wp1) /\
                      (forall x . EXC?.mrelation (c2 x) (wp2 x)) /\
                      (forall e . EXC?.mrelation (h_c e) (h_wp e))))
-          (ensures  (forall p q . wp_try_catch wp1 h_wp wp2 p q 
+          (ensures  (forall p q . wp_try_catch wp1 h_wp wp2 p q
                                   ==>
-                                  (match (rep_try_catch c1 h_c c2) with 
+                                  (match (rep_try_catch c1 h_c c2) with
                                    | Inl x -> p x
                                    | Inr e -> q e))) =
           (*(ensures  (forall p q . EXC?.mrelation (rep_try_catch c1 h_c c2) (wp_try_catch wp1 h_wp wp2))) =*)
@@ -102,14 +102,14 @@ let lemma_try_catch (#a:Type)
   | Inl x -> ()
   | Inr e -> ()
 
-let try_catch (#a:Type) 
-              (#b:Type) 
-              (#wp1:wp_type a) 
+let try_catch (#a:Type)
+              (#b:Type)
+              (#wp1:wp_type a)
               (c1:unit -> EXC a wp1)
-              (#h_wp:exn -> wp_type b) 
+              (#h_wp:exn -> wp_type b)
               (h_c:(e:exn -> EXC b (h_wp e)))
-              (#wp2:a -> wp_type b) 
-              (c2:(x:a -> EXC b (wp2 x))) 
+              (#wp2:a -> wp_type b)
+              (c2:(x:a -> EXC b (wp2 x)))
             : EXC b (wp_try_catch wp1 h_wp wp2) =
   reify_related (fun _ -> wp1) c1;
   reify_related wp2 c2;
@@ -117,48 +117,48 @@ let try_catch (#a:Type)
   lemma_try_catch #a #b wp1 (reify (c1 ())) h_wp (fun e -> reify (h_c e)) wp2 (fun x -> reify (c2 x));
   EXC?.reflect (rep_try_catch (reify (c1 ())) (fun e -> reify (h_c e)) (fun x -> reify (c2 x)))
 
-let test1 (#a:Type) 
-          (#b:Type) 
-          (#wp1:wp_type a) 
+let test1 (#a:Type)
+          (#b:Type)
+          (#wp1:wp_type a)
           (c1:unit -> EXC a wp1)
-          (#wp2:a -> wp_type b) 
-          (c2:(x:a -> EXC b (wp2 x))) 
+          (#wp2:a -> wp_type b)
+          (c2:(x:a -> EXC b (wp2 x)))
         : EXC b (wp_bind wp1 wp2) =
   try_catch #_ #_ #wp1 c1 #(fun e -> wp_raise e) (fun e -> raise e) #wp2 c2
 
-let test2 (#a:Type) 
-          (#b:Type) 
+let test2 (#a:Type)
+          (#b:Type)
           (v:a)
-          (#h_wp:exn -> wp_type b) 
+          (#h_wp:exn -> wp_type b)
           (h_c:(e:exn -> EXC b (h_wp e)))
-          (#wp2:a -> wp_type b) 
-          (c2:(x:a -> EXC b (wp2 x))) 
-        : EXC b (wp2 v) = 
+          (#wp2:a -> wp_type b)
+          (c2:(x:a -> EXC b (wp2 x)))
+        : EXC b (wp2 v) =
   try_catch #_ #_ #(wp_return v) (fun _ -> v) #h_wp h_c #wp2 c2
 
-let test3 (#a:Type) 
-          (#b:Type) 
+let test3 (#a:Type)
+          (#b:Type)
           (e:exn)
-          (#h_wp:exn -> wp_type b) 
+          (#h_wp:exn -> wp_type b)
           (h_c:(e:exn -> EXC b (h_wp e)))
-          (#wp2:a -> wp_type b) 
+          (#wp2:a -> wp_type b)
           (c2:(x:a -> EXC b (wp2 x)))
         : EXC b (h_wp e) =
   try_catch #_ #_ #(wp_raise e) (fun _ -> raise e) #h_wp h_c #wp2 c2
 
 assume val div_by_zero_exn : exn
 
-let div_wp (i j:int) = 
+let div_wp (i j:int) =
   fun p q -> (forall x . j <> 0 /\ x = i / j ==> p x) /\
              (forall e . j = 0 ==> q e)
-  
-let div (i j:int) 
+
+let div (i j:int)
   : EXC int (div_wp i j) =
   if j = 0 then raise div_by_zero_exn else i / j
 
 let try_div (i j:int)
   : EXC int (fun p q -> forall x . p x) =
-  try_catch #_ #_ 
-            #(div_wp i j) (fun _ -> div i j) 
-            #(fun _ -> wp_return 0) (fun _ -> 0) 
+  try_catch #_ #_
+            #(div_wp i j) (fun _ -> div i j)
+            #(fun _ -> wp_return 0) (fun _ -> 0)
             #(wp_return) (fun x -> x)
