examples/dm4all/ExnPartial.fst
@@ -1,0 +1,58 @@
+module ExnPartial
+
+(* Analogous to ExnTotal, but we allow exceptions and hence
+ * do partial correctness. *)
+
+let repr (a:Type) = either a exn
+
+let return (a:Type) (x:a) = Inl x
+
+let bind (a : Type) (b : Type) (l : repr a) (f : a -> repr b) =
+  match l with
+  | Inl x -> f x
+  | Inr e -> Inr e
+
+let interp (#a:Type) (l : repr a) : pure_wp a =
+    fun p -> match l with | Inl x -> p x | _ -> True
+
+total
+reifiable
+reflectable
+new_effect {
+  EXN : a:Type -> Effect
+  with
+       repr      = repr
+     ; return    = return
+     ; bind      = bind
+
+     ; wp_type   = pure_wp
+     ; return_wp = pure_return
+     ; bind_wp   = pure_bind_wp
+
+     ; interp    = interp
+}
+
+let raise (#a:Type) (e:exn) : EXN a (fun p -> True)  =
+  EXN?.reflect (Inr e)
+
+(* An alias for convenience *)
+effect Ex (a:Type) (pre:pure_pre) (post:pure_post' a pre) =
+        EXN a (fun (p:pure_post a) -> pre /\ (forall (pure_result:a). post pure_result ==> p pure_result))
+
+exception Neg
+
+let test (x:int) : EXN int (fun p -> x >= 0 /\ (forall y. p y)) =
+  if x < 0 then
+    raise Neg;
+  x + x
+
+let test' (x:int) : Ex int (requires (x >= 0)) (ensures (fun _ -> True)) =
+  if x < 0 then
+    raise Neg;
+  x + x
+
+(* This now succeeds, since raising the exception is just fine *)
+let test'' (x:int) : Ex int (requires True) (ensures (fun _ -> True)) =
+  if x < 0 then
+    raise Neg;
+  x + x
