examples/dm4all/IOForget.fst
@@ -1,7 +1,5 @@
 module IOForget
 
-open FStar.WellFounded
-
 (* Reasoning about IO without the IO: we only care about the
  * final values, and treat input as a demonic non-determistic
  * choice. *)
@@ -22,14 +20,14 @@ let return (a:Type u#a) (x:a) = Return x
 let rec bind (a : Type u#aa) (b : Type u#bb)
          (l : io a) (k : a -> io b) : io b =
   match l with
-  | Read f -> Read (fun i -> axiom1 f i; bind _ _ (f i) k)
+  | Read f -> Read (fun i -> FStar.WellFounded.axiom1 f i; bind _ _ (f i) k)
   | Write o k' -> Write o (bind _ _ k' k)
   | Return v -> k v
 
 let rec interpretation #a (m : io a) (p : pure_post a) : Type0 =
   match m with
   | Write o m -> interpretation m p
-  | Read f -> forall (i : input). (axiom1 f i ; interpretation (f i) p)
+  | Read f -> forall (i : input). (FStar.WellFounded.axiom1 f i; interpretation (f i) p)
   | Return x -> p x
 
 total
