examples/dm4all/PartialityTotal.fst
@@ -1,0 +1,59 @@
+module PartialityTotal
+
+(* Reasoning about partial programs with
+ * pure WPs, in a total correctness setting. That is,
+ * a partial program has a false precondition. *)
+
+let repr (a:Type) = option a
+
+let return (a:Type) (x:a) = Some x
+
+let bind (a : Type) (b : Type) (l : repr a) (f : a -> repr b) =
+  match l with
+  | Some x -> f x
+  | None -> None
+
+let interp (#a:Type) (l : repr a) : pure_wp a =
+    fun p -> match l with | Some x -> p x | _ -> False
+
+total
+reifiable
+reflectable
+new_effect {
+  DIV : a:Type -> Effect
+  with
+       repr      = repr
+     ; return    = return
+     ; bind      = bind
+
+     ; wp_type   = pure_wp
+     ; return_wp = pure_return
+     ; bind_wp   = pure_bind_wp
+
+     ; interp    = interp
+}
+
+let omega (#a:Type) () : DIV a (fun p -> False)  =
+  DIV?.reflect None
+
+(* An alias for convenience *)
+effect Dv (a:Type) (pre:pure_pre) (post:pure_post' a pre) =
+        DIV a (fun (p:pure_post a) -> pre /\ (forall (pure_result:a). post pure_result ==> p pure_result))
+
+let test (x:int) : DIV int (fun p -> x >= 0 /\ (forall y. p y)) =
+  if x < 0 then
+    omega ();
+  x + x
+
+let test' (x:int) : Dv int (requires (x >= 0)) (ensures (fun _ -> True)) =
+  if x < 0 then
+    omega ();
+  x + x
+
+(* This is an expected failure, since x could be negative, and this
+ * program should not verify with a trivial precondition. *)
+[@expect_failure]
+let test'' (x:int) : Dv int (requires True) (ensures (fun _ -> True)) =
+  if x < 0 then
+    omega ();
+  x + x
