examples/dm4all/St.fst
@@ -1,0 +1,83 @@
+module St
+
+(* Reasoning about state in the canonical way. *)
+
+type state = int
+
+let st a = state -> a * state
+
+let return (a:Type) (x:a) : st a = fun s -> (x, s)
+
+let bind (a b : Type) (m : st a) (f : a -> st b) : st b =
+  fun s -> let (v, s') = m s in f v s'
+
+let post a = a -> state -> Type0
+let wpty a = state -> post a -> Type0
+
+let return_wp (a:Type) (x:a) : wpty a =
+  fun h p -> p x h
+
+unfold
+let bind_wp (_ : range) (a:Type) (b:Type) (w : wpty a) (kw : a -> wpty b) : wpty b =
+  fun h p -> w h (fun x h' -> kw x h' (fun y h'' -> p y h''))
+
+let interpretation #a (m : st a) (s0 : state) (p : post a) : Type0 =
+  let (x, s1) = m s0 in p x s1
+
+total
+reifiable
+reflectable
+new_effect {
+  St : a:Type -> Effect
+  with
+       repr      = st
+     ; return    = return
+     ; bind      = bind
+
+     ; wp_type   = wpty
+     ; return_wp = return_wp
+     ; bind_wp   = bind_wp
+
+     ; interp    = interpretation
+}
+
+(* Actions *)
+val get : unit -> St state (fun s p -> p s s)
+let get () =
+  St?.reflect (fun s -> (s,s))
+
+val set : s:state -> St unit (fun _ p -> p () s)
+let set s =
+  St?.reflect (fun _ -> ((), s))
+
+val modify (f : state -> state) : St unit (fun s p -> p () (f s))
+let modify f =
+    let s = get () in
+    set (f s)
+
+let test1 () : St int (fun s0 p -> p 42 (s0 + 5)) =
+  let x = get () in
+  set (x + 2);
+  let y = get () in
+  set (y + 3);
+  42
+
+let test2 () : St int (fun s0 p -> s0 >= 1 /\ p (s0 + 2) (s0 + 5)) =
+  let x = get () in
+  set (x + 2);
+  let y = get () in
+  set (y + 3);
+  y
+
+let test3 () : St int (fun s0 p -> forall x s1. p x s1) =
+  let x = get () in
+  set (1 + x `op_Multiply` x);
+  test2 ()
+  
+(* This fails since we cannot prove test2's precondition,
+ * i.e. that the state is >= 1 *)
+[@expect_failure]
+let test4 () : St int (fun s0 p -> forall x s1. p x s1) =
+  let x = get () in
+  set (x `op_Multiply` x);
+  test2 ()
