examples/dm4all/StExnPartial.fst
@@ -1,0 +1,85 @@
+module StExnPartial
+
+(* Reasoning about State plus exceptions, but WPs only over
+ * the stateful part. Exceptions are all taken as success, i.e.,
+ * we consider partial correctness only. *)
+
+type state = int
+
+let st a = state -> option (a * state)
+
+let return (a:Type) (x:a) : st a = fun s -> Some (x, s)
+
+let bind (a b : Type) (m : st a) (f : a -> st b) : st b =
+  fun s -> match m s with
+        | Some (v, s') -> f v s'
+        | None -> None
+
+let post a = a -> state -> Type0
+let wpty a = state -> post a -> Type0
+
+let return_wp (a:Type) (x:a) : wpty a =
+  fun h p -> p x h
+
+unfold
+let bind_wp (_ : range) (a:Type) (b:Type) (w : wpty a) (kw : a -> wpty b) : wpty b =
+  fun h p -> w h (fun x h' -> kw x h' (fun y h'' -> p y h''))
+
+let interpretation #a (m : st a) (s0 : state) (p : post a) : Type0 =
+  match m s0 with
+  | Some (x, s1) -> p x s1
+  | None -> True
+
+total
+reifiable
+reflectable
+new_effect {
+  StExn : a:Type -> Effect
+  with
+       repr      = st
+     ; return    = return
+     ; bind      = bind
+
+     ; wp_type   = wpty
+     ; return_wp = return_wp
+     ; bind_wp   = bind_wp
+
+     ; interp    = interpretation
+}
+
+(* Actions *)
+val get : unit -> StExn state (fun s p -> p s s)
+let get () =
+  StExn?.reflect (fun s -> Some (s,s))
+
+val set : s:state -> StExn unit (fun _ p -> p () s)
+let set s =
+  StExn?.reflect (fun _ -> Some ((), s))
+
+let raise () : StExn unit (fun _ _ -> True) =
+  StExn?.reflect (fun s -> None)
+
+let test1 () : StExn int (fun s0 p -> p 42 (s0 + 5)) =
+  let x = get () in
+  set (x + 2);
+  let y = get () in
+  set (y + 3);
+  42
+
+(* This can raise an exception, since the initial state could be < 1,
+ * but since we're doing partial correctness it is accepted *)
+let test2 () : StExn int (fun s0 p -> p 42 (s0 + 5)) =
+  let x = get () in
+  if x < 1 then raise ();
+  set (x + 2);
+  let y = get () in
+  set (y + 3);
+  42
+
+let test3 () : StExn int (fun s0 p -> s0 >= 1 /\ p (s0 + 2) (s0 + 5)) =
+  let x = get () in
+  if x < 1 then raise ();
+  set (x + 2);
+  let y = get () in
+  set (y + 3);
+  y
